lean/src/internal/redundant_leaves_can_be_removed_2/inactive.lean
@@ -7,6 +7,7 @@ import data.list
 import data.bool
 import ..leaves_theory
 import ..gdt_eval
+import ..gdt_eval_option
 
 open finset
 
@@ -58,10 +59,12 @@ end
 def Gdt.mark_inactive_leaves : Gdt → Env → Ant bool
 | (Gdt.leaf leaf) env := Ant.leaf ff leaf 
 | (Gdt.branch tr1 tr2) env :=
-    if (tr1.eval env).is_match then
-        Ant.branch (tr1.mark_inactive_leaves env) (tr2.mark_all_leaves_inactive)
-    else
-        Ant.branch (tr1.mark_all_leaves_inactive) (tr2.mark_inactive_leaves env)
+    Ant.branch (tr1.mark_inactive_leaves env) (
+        if (tr1.eval env).is_match then
+            (tr2.mark_all_leaves_inactive)
+        else
+            (tr2.mark_inactive_leaves env)
+    )
 | (Gdt.grd (Grd.xgrd grd) tr) env :=
     match xgrd_eval grd env with
     | none := tr.mark_all_leaves_inactive
@@ -163,6 +166,68 @@ begin
     tauto, 
 end
 
+lemma redundant_in_mark_all_leaves_inactive (gdt: Gdt) (leaves: finset Leaf): leaves.redundant_in gdt.mark_all_leaves_inactive :=
+begin
+    unfold redundant_in,
+    simp [inter_subset_right],
+end
+
+lemma sets_3 { α: Type } [decidable_eq α] { a b c : finset α }
+  (h : ¬ a ∪ b ⊆ c):
+  ¬a ⊆ c ∨ ¬b ⊆ c :=
+begin
+    by_contra x,
+    push_neg at x,
+    have : a ∪ b ⊆ c :=
+    begin
+        rw finset.subset_iff,
+        simp,
+        rw finset.subset_iff at x,
+        rw finset.subset_iff at x,
+        tauto,
+    end,
+    contradiction,
+end
+
+lemma remove_leaves_branch { leaves: finset Leaf } { gdt₁ gdt₂: Gdt }:
+    (gdt₁.branch gdt₂).remove_leaves leaves ≠ none ↔
+         gdt₁.remove_leaves leaves ≠ none ∨
+         gdt₂.remove_leaves leaves ≠ none :=
+begin
+    unfold Gdt.remove_leaves,
+    cases gdt₁.remove_leaves leaves;
+    cases gdt₂.remove_leaves leaves;
+    simp [Gdt.branch_option],
+end
+
+lemma Gdt.grd_option_neq_none { gdt: option Gdt } { grd: Grd }: Gdt.grd_option grd gdt ≠ none ↔ gdt ≠ none :=
+begin
+    cases gdt;
+    simp [Gdt.grd_option],
+end
+
+lemma remove_leaves_neq_none { leaves: finset Leaf } { gdt: Gdt } (h: ¬ gdt.leaves ⊆ leaves): (Gdt.remove_leaves leaves gdt) ≠ none :=
+begin
+    induction gdt with leaf,
+    case Gdt.leaf {
+        simp only [Gdt.leaves, singleton_subset_iff] at h,
+        simp [Gdt.remove_leaves, h],
+    },
+    case Gdt.branch {
+        simp only [Gdt.leaves] at h,
+        rw remove_leaves_branch,
+        have := sets_3 h,
+        cases this;
+        simp [*],
+    },
+    case Gdt.grd {
+        unfold Gdt.remove_leaves,
+        unfold Gdt.leaves at h,
+        rw Gdt.grd_option_neq_none,
+        simp [gdt_ih h],
+    }
+end
+
 lemma redundant_leaves_removable
     (gdt: Gdt) (gdt_disjoint: gdt.disjoint_leaves)
     -- We only focus on a very particular environment `env`.
@@ -175,19 +240,29 @@ begin
   case Gdt.leaf {
       simp [Gdt.eval],
       unfold Gdt.mark_inactive_leaves finset.redundant_in at leaves_def,
-      simp [Ant.inactive_leaves, Ant.critical_leaf_sets] at leaves_def,
-      sorry,
+      simp [Ant.inactive_leaves, Ant.critical_leaf_sets, Ant.leaves] at leaves_def,
+      unfold Gdt.remove_leaves,
+      have : ¬leaf ∈ leaves := disjoint_singleton.mp leaves_def,
+      simp [this, Gdt.eval_option],
   },
 
   case Gdt.branch {
         simp [Gdt.mark_inactive_leaves, -Result.is_match_neq_no_match] at leaves_def,
-        cases (gdt_tr1.eval env).is_match,
-        case bool.ff {
-            simp [Ant.inactive_leaves, Gdt.mark_inactive_leaves, finset.redundant_in, Ant.critical_leaf_sets ] at leaves_def,
-            simp [Ant.leaves] at leaves_def,
+        unfold Gdt.remove_leaves,
+        unfold Gdt.disjoint_leaves at gdt_disjoint,
 
-            unfold Gdt.remove_leaves,
-            unfold Gdt.disjoint_leaves at gdt_disjoint,
+        cases c: (gdt_tr1.eval env).is_match,
+        
+        case bool.ff {
+            rw c at leaves_def,
+            simp at c,
+            simp [Ant.inactive_leaves, Gdt.mark_inactive_leaves, finset.redundant_in, Ant.critical_leaf_sets ] at leaves_def,
+            simp [Ant.leaves, Gdt.mark_inactive_leaves_no_match c] at leaves_def,
+
+            have : leaves.redundant_in (gdt_tr1.mark_inactive_leaves env) :=
+            by simp [Gdt.mark_inactive_leaves_no_match c, redundant_in_mark_all_leaves_inactive],
+
+            specialize gdt_ih_tr1 gdt_disjoint.1 env this,
 
             have : leaves.redundant_in (gdt_tr2.mark_inactive_leaves env) :=
             begin
@@ -198,14 +273,17 @@ begin
             end,
 
             specialize gdt_ih_tr2 gdt_disjoint.2.1 env this,
-            sorry,
+            rw ←Gdt.eval_option at gdt_ih_tr2,
+            rw Gdt.branch_option_replace_right_env _ (or.intro_left _ gdt_ih_tr2),
+            rw ←Gdt.eval_option at gdt_ih_tr1,
+            rw Gdt.branch_option_replace_left_env gdt_ih_tr1,
+            simp,
         },
         case bool.tt {
+            rw c at leaves_def,
+            simp at c,
             simp [Ant.inactive_leaves, Gdt.mark_inactive_leaves, redundant_in, Ant.critical_leaf_sets ] at leaves_def,
             simp [Ant.leaves] at leaves_def,
-
-            unfold Gdt.remove_leaves,
-            unfold Gdt.disjoint_leaves at gdt_disjoint,
 
             have : leaves.redundant_in (gdt_tr1.mark_inactive_leaves env) :=
             begin
@@ -216,7 +294,12 @@ begin
                 exact leaves_def.2,
             end,
             specialize gdt_ih_tr1 gdt_disjoint.1 env this,
-            sorry,
+            rw ←Gdt.eval_option at c,
+            
+            rw ←Gdt.eval_option at gdt_ih_tr1,
+            rw Gdt.branch_option_replace_left_env gdt_ih_tr1,
+            rw Gdt.branch_option_replace_right_env (some gdt_tr2) (or.intro_right _ c),
+            simp,
         },
     },
 
@@ -237,12 +320,13 @@ begin
                 
                 specialize gdt_ih gdt_disjoint env' this,
                 unfold Gdt.remove_leaves,
-                sorry,
+                rw Gdt.eval_option_of_xgrd_eval_some c,
+                exact gdt_ih,
             },
             case option.none {
                 simp [grd_eval_xgrd_none c],
                 unfold Gdt.remove_leaves,
-                sorry,
+                exact Gdt.eval_option_of_xgrd_eval_none c,
             },
         },
         case Grd.bang {
@@ -251,7 +335,7 @@ begin
                 simp [grd_eval_bang_bottom c],
                 simp [redundant_in, Gdt.leaves, Ant.leaves, Ant.inactive_leaves, Ant.critical_leaf_sets, Gdt.mark_inactive_leaves, c] at leaves_def,
                 unfold Gdt.remove_leaves,
-                sorry,
+                apply Gdt.eval_option_of_is_bottom_tt c (remove_leaves_neq_none leaves_def.2),
             },
             case bool.ff {
                 simp [redundant_in, Gdt.leaves, Gdt.mark_inactive_leaves, c, Ant.leaves, Ant.inactive_leaves, Ant.critical_leaf_sets] at leaves_def,
@@ -262,7 +346,8 @@ begin
                 specialize gdt_ih gdt_disjoint env this,
                 unfold Gdt.remove_leaves,
                 simp [grd_eval_bang_not_bottom c],
-                sorry,
+                rw Gdt.eval_option_of_is_bottom_ff c,
+                exact gdt_ih,
             },
         },
     },
