lean/src/internal/gdt_eval_option.lean
@@ -1,0 +1,68 @@
+import tactic
+import .gdt_eval
+import ..definitions
+
+variable [GuardModule]
+open GuardModule
+
+lemma Gdt.branch_option_replace_left_env { gdt₁ gdt₁' gdt₂: option Gdt } { env: Env }
+    (h: Gdt.eval_option gdt₁ env = Gdt.eval_option gdt₁' env):
+    Gdt.eval_option (Gdt.branch_option gdt₁ gdt₂) env = Gdt.eval_option (Gdt.branch_option gdt₁' gdt₂) env :=
+by cases gdt₁; cases gdt₁'; cases gdt₂; finish [Gdt.branch_option, Gdt.eval_option, Gdt.eval, gdt_eval_branch_left_no_match]
+
+lemma Gdt.branch_option_replace_right_env { gdt₁ gdt₂: option Gdt } (gdt₂': option Gdt) { env: Env }
+    (h: Gdt.eval_option gdt₂ env = Gdt.eval_option gdt₂' env ∨ Gdt.eval_option gdt₁ env ≠ Result.no_match):
+    Gdt.eval_option (Gdt.branch_option gdt₁ gdt₂) env = Gdt.eval_option (Gdt.branch_option gdt₁ gdt₂') env :=
+begin
+  cases gdt₁;
+  cases gdt₂;
+  cases gdt₂',
+
+  
+  finish [Gdt.branch_option, Gdt.eval_option, Gdt.eval, gdt_eval_branch_left_no_match],
+  finish [Gdt.branch_option, Gdt.eval_option, Gdt.eval, gdt_eval_branch_left_no_match],
+  finish [Gdt.branch_option, Gdt.eval_option, Gdt.eval, gdt_eval_branch_left_no_match],
+  finish [Gdt.branch_option, Gdt.eval_option, Gdt.eval, gdt_eval_branch_left_no_match],
+  finish [Gdt.branch_option, Gdt.eval_option, Gdt.eval, gdt_eval_branch_left_no_match],
+
+  simp [Gdt.branch_option, Gdt.eval_option, gdt_eval_branch_left_no_match],
+  simp [Gdt.branch_option, Gdt.eval_option, gdt_eval_branch_left_no_match] at h,
+  rw gdt_eval_branch_right_no_match2,
+  finish,
+  
+
+  simp [Gdt.branch_option, Gdt.eval_option, gdt_eval_branch_left_no_match],
+  simp [Gdt.branch_option, Gdt.eval_option, gdt_eval_branch_left_no_match] at h,
+  rw gdt_eval_branch_right_no_match2,
+  finish,
+  
+
+  simp [Gdt.branch_option, Gdt.eval_option, gdt_eval_branch_left_no_match],
+  simp [Gdt.branch_option, Gdt.eval_option, gdt_eval_branch_left_no_match] at h,
+  exact Gdt.branch_replace_right_env h,
+end
+
+@[simp]
+lemma Gdt.eval_option_branch_option_some (gdt₁ gdt₂: Gdt) (env: Env):
+  Gdt.eval_option (Gdt.branch_option (some gdt₁) (some gdt₂)) env = (gdt₁.branch gdt₂).eval env :=
+by simp [Gdt.branch_option, Gdt.eval_option]
+
+lemma Gdt.eval_option_of_xgrd_eval_some { grd: XGrd } { tr: option Gdt } { env env': Env }
+    (h: xgrd_eval grd env = some env'):
+    Gdt.eval_option (Gdt.grd_option (Grd.xgrd grd) tr) env = Gdt.eval_option tr env' :=
+by cases tr; simp [Gdt.eval_option, Gdt.grd_option, grd_eval_xgrd_some h, *]
+
+lemma Gdt.eval_option_of_xgrd_eval_none { grd: XGrd } { tr: option Gdt } { env: Env }
+    (h: xgrd_eval grd env = none):
+    Gdt.eval_option (Gdt.grd_option (Grd.xgrd grd) tr) env = Result.no_match :=
+by cases tr; simp [Gdt.eval_option, Gdt.grd_option, grd_eval_xgrd_none h, *]
+
+lemma Gdt.eval_option_of_is_bottom_ff { var: Var } { tr: option Gdt } { env: Env }
+  (h: is_bottom var env = ff):
+    Gdt.eval_option (Gdt.grd_option (Grd.bang var) tr) env = Gdt.eval_option tr env :=
+by cases tr; simp [Gdt.grd_option, Gdt.eval_option, grd_eval_bang_not_bottom h]
+
+lemma Gdt.eval_option_of_is_bottom_tt { var: Var } { tr: option Gdt } { env: Env }
+  (h: is_bottom var env = tt) (g: tr ≠ none):
+    Gdt.eval_option (Gdt.grd_option (Grd.bang var) tr) env = Result.diverged :=
+by cases tr; finish [Gdt.grd_option, Gdt.eval_option, Gdt.eval, h]
