lean/src/internal/redundant_leaves_can_be_removed_2/main.lean
@@ -26,8 +26,8 @@ lemma Ant.mark_inactive_leaves.diverge (a) (ant: Ant Φ) (env) :
     (Ant.diverge a ant).mark_inactive_leaves env = Ant.diverge (!(a.eval env)) (ant.mark_inactive_leaves env) :=
 by simp [Ant.map, Ant.mark_inactive_leaves]
 
-lemma can_prove_empty_implies_inactive { can_prove_empty: Gs } { ant: Ant Φ } { env: Env }:
-    (ant.map (can_prove_empty.val)) ⇒ (ant.mark_inactive_leaves env) :=
+lemma can_prove_empty_implies_inactive (can_prove_empty: Gs) (ant: Ant Φ) (env: Env):
+    (ant.map (can_prove_empty.val)) ⟶ (ant.mark_inactive_leaves env) :=
 begin
     induction ant,
     case Ant.leaf {
@@ -72,13 +72,12 @@ begin
 
         cases c: (gdt_tr1.eval env).is_match,
         case bool.ff {
-            have : gdt_tr1.eval env = Result.no_match, { cases gdt_tr1.eval env; finish, },
             specialize gdt_ih_tr1 env,
             unfold Ant.mark_inactive_leaves at gdt_ih_tr1,
             specialize gdt_ih_tr2 env,
             unfold Ant.mark_inactive_leaves at gdt_ih_tr2,
             
-            simp [c, ←Gdt.mark_inactive_leaves_no_match this, *],
+            simp [c, ←Gdt.mark_inactive_leaves_no_match, *],
         },
 
         case bool.tt {
@@ -150,7 +149,7 @@ begin
     },
 end
 
-lemma redundant_in.monotonous' { a b: Ant bool } (h: a ⇒ b): 
+lemma redundant_in.monotonous' { a b: Ant bool } (h: a ⟶ b): 
         a.inactive_leaves ⊆ b.inactive_leaves ∧ b.critical_leaf_sets ⊆ a.critical_leaf_sets :=
 begin
     induction a generalizing b;
@@ -182,7 +181,7 @@ begin
     },
 end
 
-lemma redundant_in.monotonous { a b: Ant bool } (leaves: finset Leaf) (h: a ⇒ b):
+lemma redundant_in.monotonous { a b: Ant bool } (leaves: finset Leaf) (h: a ⟶ b):
     leaves.redundant_in a → leaves.redundant_in b :=
 begin
     unfold finset.redundant_in,
@@ -196,6 +195,200 @@ begin
     assume e,
     assume q,
     exact p.right e (this.2 q),
+end
+
+lemma disjoint_finset { α: Type } [decidable_eq α] { a b: list α } (d : disjoint a.to_finset b.to_finset) : a.disjoint b :=
+begin
+    unfold list.disjoint,
+    assume x h₁ h₂,
+    finish [finset.disjoint_iff_ne],
+end
+
+theorem card_insert_iff_not_mem { α: Type } [decidable_eq α] {a : α} {s : finset α}: (insert a s).card = s.card + 1 ↔ a ∉ s :=
+begin
+    split,
+    {
+        assume h,
+        by_contra,
+        finish [finset.card_insert_of_mem, s.card.succ_ne_self.symm],
+    },
+    { exact finset.card_insert_of_not_mem, },
+end
+
+theorem nodup_iff_card { α: Type } [decidable_eq α] (a: list α): a.nodup ↔ a.length = a.to_finset.card :=
+begin
+    split; assume h,
+    { simp [list.to_finset_card_of_nodup h], },
+
+    induction a with a as,
+    case list.nil { simp, },
+    case list.cons {
+        rw list.nodup_cons,
+        replace h : as.length + 1 = (insert a as.to_finset).card := begin
+            simp at h,
+            exact h,
+        end,
+        by_cases a ∈ as.to_finset, {
+            replace h : as.length + 1 = as.to_finset.card, { simp [*], },
+            have y := list.to_finset_card_le as,
+            rw ←h at y,
+            simp at y,
+            contradiction,
+        }, {
+            replace x : as.length = as.to_finset.card, { finish, },
+            finish,
+        }
+    },
+end 
+
+example {α} [decidable_eq α] (as bs cs ds : list α) : (as ++ bs ++ cs ++ ds).nodup ↔ (ds ++ bs ++ cs ++ as).nodup :=
+begin
+  rw nodup_iff_card,
+  rw nodup_iff_card,
+  simp [finset.union_comm, finset.union_left_comm, nat.add_comm, nat.add_left_comm],
+end
+
+lemma R_red_partition' { ant: Ant bool } (ant_disjoint: ant.disjoint_leaves):
+    ((R ant).acc ++ (R ant).inacc ++ (R ant).red).to_finset = ant.leaves ∧ 
+    ((R ant).acc ++ (R ant).inacc ++ (R ant).red).length = ant.leaves.card :=
+begin
+    induction ant,
+    case Ant.leaf {
+        unfold R,
+        cases ant_a;
+        simp [Ant.leaves, R],
+    },
+    case Ant.branch {
+        unfold Ant.disjoint_leaves at ant_disjoint,
+        specialize ant_ih_tr1 ant_disjoint.1,
+        specialize ant_ih_tr2 ant_disjoint.2.1,
+        
+        unfold R,
+        dsimp only,
+        unfold Ant.leaves,
+        split, {
+            simp [←ant_ih_tr1.1, ←ant_ih_tr2.1, finset.union_comm, finset.union_assoc, finset.union_left_comm],
+        },
+
+        rw finset.card_disjoint_union ant_disjoint.2.2,
+        simp [←ant_ih_tr1.2, ←ant_ih_tr2.2, nat.add_comm, nat.add_assoc, nat.add_left_comm],
+    },
+    case Ant.diverge {
+        unfold Ant.disjoint_leaves at ant_disjoint,
+        specialize ant_ih ant_disjoint,
+        cases R_diverge_cases ant_tr ant_a, {
+            rw h_R,
+            unfold LeafPartition.acc LeafPartition.inacc LeafPartition.red Ant.leaves,
+            rw h_R_ant at ant_ih,
+            unfold LeafPartition.acc LeafPartition.inacc LeafPartition.red Ant.leaves at ant_ih,
+            simp at ant_ih,
+            simp [*],
+        }, {
+            rw h_R,
+            exact ant_ih,
+        },
+    }
+end
+
+lemma R_red_partition { ant: Ant bool } (ant_disjoint: ant.disjoint_leaves):
+    ((R ant).acc ++ (R ant).inacc ++ (R ant).red).to_finset = ant.leaves ∧ 
+    ((R ant).acc ++ (R ant).inacc ++ (R ant).red).nodup :=
+begin
+    rw nodup_iff_card,
+    rw (R_red_partition' ant_disjoint).1,
+    rw (R_red_partition' ant_disjoint).2,
+    simp,
+end    
+
+
+/-
+lemma R_red_partition2 { ant: Ant bool } (ant_disjoint: ant.disjoint_leaves):
+    ((R ant).acc ++ (R ant).inacc ++ (R ant).red).to_finset = ant.leaves ∧ 
+    ((R ant).acc ++ (R ant).inacc ++ (R ant).red).nodup :=
+begin
+    induction ant,
+    case Ant.leaf {
+        unfold R,
+        cases ant_a;
+        simp [Ant.leaves, R],
+    },
+    case Ant.branch {
+        unfold Ant.disjoint_leaves at ant_disjoint,
+        specialize ant_ih_tr1 ant_disjoint.1,
+        specialize ant_ih_tr2 ant_disjoint.2.1,
+        
+        unfold R,
+        unfold LeafPartition.acc LeafPartition.inacc LeafPartition.red Ant.leaves,
+        split, { finish, },
+
+        suffices : (((R ant_tr1).acc ++ (R ant_tr1).inacc ++ (R ant_tr1).red)
+            ++ ((R ant_tr2).acc ++ (R ant_tr2).inacc ++ (R ant_tr2).red)).nodup, {
+            rw list.nodup_append_comm
+            
+        },
+
+        apply list.nodup_append.2,
+        split, { exact ant_ih_tr1.2, },
+        split, { exact ant_ih_tr2.2, },
+
+        have d := ant_disjoint.2.2,
+        rw ←ant_ih_tr1.1 at d,
+        rw ←ant_ih_tr2.1 at d,
+        
+        apply disjoint_finset d,
+    },
+    case Ant.diverge {
+        sorry,
+    }
+end
+-/
+
+lemma R_red_l_not_mem_ls { ant: Ant bool } (ant_disjoint: ant.disjoint_leaves) { l: Leaf } { ls: list Leaf } (h: (R ant).red = l::ls):
+    l ∉ ls.to_finset :=
+begin
+    have : (R ant).red.nodup := begin
+        exact list.nodup_of_nodup_append_right (R_red_partition ant_disjoint).2,
+    end,
+    rw h at this,
+    simp [list.not_mem_of_nodup_cons this],
+end
+
+lemma R_acc_l_not_mem { ant: Ant bool } (ant_disjoint: ant.disjoint_leaves) { l: Leaf } { ls: list Leaf } (h: (R ant).acc = l::ls):
+    l ∉ (R ant).red.to_finset :=
+begin
+    have d := list.disjoint_of_nodup_append (R_red_partition ant_disjoint).2,
+    have : l ∈ ((R ant).acc ++ (R ant).inacc) := by simp [h],
+    suffices : l ∉ (R ant).red, { simp [this], },
+    exact imp_false.mp (@d l this),
+end
+
+lemma R_inacc_l_not_mem { ant: Ant bool } (ant_disjoint: ant.disjoint_leaves) { l: Leaf } { ls: list Leaf } (h: (R ant).inacc = l::ls):
+    l ∉ (R ant).red.to_finset :=
+begin
+    have d := list.disjoint_of_nodup_append (R_red_partition ant_disjoint).2,
+    have : l ∈ ((R ant).acc ++ (R ant).inacc) := by simp [h],
+    suffices : l ∉ (R ant).red, { simp [this], },
+    exact imp_false.mp (@d l this),
+end
+
+lemma R_acc_subset_leaves { ant: Ant bool } (ant_disjoint: ant.disjoint_leaves): (R ant).acc.to_finset ⊆ ant.leaves :=
+begin
+    have := (R_red_partition ant_disjoint).1,
+    replace this := finset.subset_of_eq this,
+    rw finset.subset_iff at this,
+    simp at this,
+    rw finset.subset_iff,
+    finish,
+end
+
+lemma R_inacc_subset_leaves { ant: Ant bool } (ant_disjoint: ant.disjoint_leaves): (R ant).inacc.to_finset ⊆ ant.leaves :=
+begin
+    have := (R_red_partition ant_disjoint).1,
+    replace this := finset.subset_of_eq this,
+    rw finset.subset_iff at this,
+    simp at this,
+    rw finset.subset_iff,
+    finish,
 end
 
 lemma R_red_subset_leaves { ant: Ant bool }: (R ant).red.to_finset ⊆ ant.leaves :=
@@ -221,6 +414,29 @@ begin
     },
 end
 
+lemma critical_leaf_set_elements { ant: Ant bool } { e: finset Leaf } (h: e ∈ ant.critical_leaf_sets):
+    e ⊆ ant.leaves :=
+begin
+    induction ant;
+    rw Ant.critical_leaf_sets at h,
+    case Ant.leaf {
+        finish,
+    },
+    case Ant.branch {
+        simp at h,
+        cases h;
+        simp [Ant.leaves, subset_right_union, subset_left_union, *],
+    },
+    case Ant.diverge {
+        simp at h,
+        cases h;
+        try {
+            cases ant_a;
+            finish [Ant.leaves],
+        },
+    },
+end
+
 lemma subset_inter_subset { α: Type } [decidable_eq α] { s1 s2 s3: finset α }: s1 ⊆ s3 → s1 ∩ s2 ⊆ s3 :=
 begin
     refine finset.subset.trans _,
@@ -238,7 +454,55 @@ begin
     },
 end
 
-lemma R_red_redundant (ant: Ant bool)
+lemma not_subset { α: Type } { u v: finset α }: ¬ u ⊆ v ↔ ∃ x ∈ u, ¬ x ∈ v :=
+begin
+    exact not_ball
+end
+
+lemma Ant.leaves_non_empty { α: Type } (ant: Ant α) : ∃ l, l ∈ ant.leaves :=
+begin
+    induction ant,
+    case Ant.leaf { simp [Ant.leaves], },
+    case Ant.diverge { simp [Ant.leaves, *], },
+    case Ant.branch {
+        cases ant_ih_tr1 with leaf,
+        use leaf,
+        simp [Ant.leaves, *],
+    }
+end
+
+@[simp]
+lemma Ant.disjoint_leaves_of_map { α β: Type } { f: α → β } { ant: Ant α }: (ant.map f).disjoint_leaves ↔ ant.disjoint_leaves :=
+by induction ant; { simp [Ant.map, Ant.disjoint_leaves, *], }
+
+lemma Ant.disjoint_leaves_of_mark_inactive_leaves_eq { ant1 ant2: Ant Φ } { env: Env } (h: ant1.mark_inactive_leaves env = ant2.mark_inactive_leaves env):
+    ant1.disjoint_leaves ↔ ant2.disjoint_leaves :=
+begin
+    unfold Ant.mark_inactive_leaves at h,
+    have : (Ant.map (λ (ty : Φ), !ty.eval env) ant1).disjoint_leaves ↔ (Ant.map (λ (ty : Φ), !ty.eval env) ant2).disjoint_leaves :=
+    begin
+        simp [h],
+    end,
+    simp at this,
+    exact this,
+end
+
+lemma Ant.disjoint_leaves_of_gdt_disjoint_leaves { gdt: Gdt } (h: gdt.disjoint_leaves): (A gdt).disjoint_leaves :=
+begin
+    induction gdt,
+    case Gdt.leaf { simp [A], },
+    case Gdt.branch {
+        unfold Gdt.disjoint_leaves at h,
+        simp [A, Gdt.disjoint_leaves, Ant.disjoint_leaves, *],
+    },
+    case Gdt.grd {
+        unfold Gdt.disjoint_leaves at h,
+        cases gdt_grd;
+        { simp [A, Ant.disjoint_leaves, *], },
+    },
+end
+
+lemma R_red_redundant { ant: Ant bool }
     (ant_disjoint: ant.disjoint_leaves)
     : (R ant).red.to_finset.redundant_in ant :=
 begin
@@ -272,15 +536,54 @@ begin
         assume h,
         rw Ant.critical_leaf_sets at h,
         
-        simp,
+        simp [Ant.leaves],
         replace ant_ih_tr1 := ant_ih_tr1.2,
         replace ant_ih_tr2 := ant_ih_tr2.2,
-        sorry,
+        simp at h,
+        cases h, {
+            specialize ant_ih_tr1 e h,
+            rw not_subset,
+            rw not_subset at ant_ih_tr1,
+            cases ant_ih_tr1 with x ant_ih_tr1,
+            cases ant_ih_tr1 with H ant_ih_tr1,
+            
+            have : x ∉ (R ant_tr2).red.to_finset :=
+            begin
+                by_contradiction,
+                have h1 := finset.subset_iff.1 (critical_leaf_set_elements h) H,
+                have h2 := finset.subset_iff.1 (R_red_subset_leaves) a,
+                have := finset.disjoint_iff_ne.1 ant_disjoint.2.2 _ h1 _ h2,
+                simp at this,
+                exact this,
+            end,
+            use x,
+            simp [*],
+        },  
+        {
+            specialize ant_ih_tr2 e h,
+            rw not_subset,
+            rw not_subset at ant_ih_tr2,
+            cases ant_ih_tr2 with x ant_ih_tr2,
+            cases ant_ih_tr2 with H ant_ih_tr2,
+            
+            have : x ∉ (R ant_tr1).red.to_finset :=
+            begin
+                by_contradiction,
+                have h1 := finset.subset_iff.1 (critical_leaf_set_elements h) H,
+                have h2 := finset.subset_iff.1 (R_red_subset_leaves) a,
+                have := finset.disjoint_iff_ne.1 ant_disjoint.2.2 _ h2 _ h1,
+                simp at this,
+                exact this,
+            end,
+            use x,
+            simp [*],
+        }
     },
     case Ant.diverge {
         unfold finset.redundant_in,
         unfold finset.redundant_in at ant_ih,
-
+        unfold Ant.disjoint_leaves at ant_disjoint,
+        specialize ant_ih ant_disjoint,
         split, {
             cases R_diverge ant_a (refl (R ant_tr)) with d d,
             case or.inl {
@@ -291,11 +594,15 @@ begin
                 rw d.2.1 at ant_ih,
                 unfold LeafPartition.red at ant_ih,
                 unfold Ant.inactive_leaves,
-                sorry,
+                unfold Ant.leaves,
+                have : ls.to_finset ⊆ (leaf :: ls).to_finset := by simp [finset.subset_insert],
+                have := finset.inter_subset_inter this (finset.subset.refl _),
+                exact finset.subset.trans this ant_ih.1,
             },
             case or.inr {
                 simp [d.2, Ant.inactive_leaves, ant_ih.1],
-                sorry,
+                unfold Ant.leaves,
+                exact ant_ih.1,
             },
         },
 
@@ -307,8 +614,54 @@ begin
 
         cases R_diverge ant_a (refl (R ant_tr)) with d d,
         case or.inr {
-            rw d.2,
-            sorry,
+            cases d,
+            rw d_right,
+            cases ant_a,
+            case bool.tt {
+                simp [d_left] at h,
+                exact ant_ih.2 e h,
+            },
+            simp at h,
+            cases h, { exact ant_ih.2 e h, },
+            rw h,
+            cases d_left, {
+                finish,
+            },
+            cases d_left, {
+                rw not_subset,
+                cases c: (R ant_tr).acc with acc accs, { finish, },
+                use acc,
+                split, {
+                    have x : acc ∈ (R ant_tr).acc.to_finset := by simp [c],
+                    have := R_acc_subset_leaves ant_disjoint,
+                    rw finset.subset_iff at this,
+                    exact @this acc x,
+                }, {
+                    exact R_acc_l_not_mem ant_disjoint c,
+                },
+            },
+            cases d_left, {
+                rw not_subset,
+                cases c: (R ant_tr).inacc with inacc inaccs, { finish, },
+                use inacc,
+                split, {
+                    have x : inacc ∈ (R ant_tr).inacc.to_finset := by simp [c],
+                    have := R_inacc_subset_leaves ant_disjoint,
+                    rw finset.subset_iff at this,
+                    exact @this inacc x,
+                }, {
+                    exact R_inacc_l_not_mem ant_disjoint c,
+                },
+            },
+            {
+                rw not_subset,
+                have := Ant.leaves_non_empty ant_tr,
+                cases this with l ls,
+                rw d_left,
+                use l,
+                split, { exact ls, },
+                simp,
+            }
         },
 
         case or.inl {
@@ -320,53 +673,281 @@ begin
             unfold LeafPartition.red,
             rw d.2.1 at ant_ih,
             unfold LeafPartition.red at ant_ih,
-            sorry,
+            rw not_subset,
+            have := ant_ih.2 e,
+            rw not_subset at this,
+            cases h, {
+                specialize this h,
+                cases this with x this,
+                cases this with H this,
+                use x,
+                simp at this,
+                finish,
+            }, {
+                use leaf,
+                rw h,
+                have : leaf ∈ (R ant_tr).red.to_finset := by simp [*],
+                have := finset.subset_iff.1 R_red_subset_leaves this,
+                split, { exact this, },
+                apply R_red_l_not_mem_ls ant_disjoint,
+                rw d.2.1,
+            }
         },
     },
 end
 
 theorem R_red_removable
     (can_prove_empty: Gs)
-    (gdt: Gdt) (gdt_disjoint: gdt.disjoint_leaves):
-    Gdt.eval_option (gdt.remove_leaves ((R $ (A gdt).map can_prove_empty.val).red.to_finset)) = gdt.eval :=
+    (gdt: Gdt) (gdt_disjoint: gdt.disjoint_leaves)
+    (Agdt: Ant Φ)
+    (ant_def: Agdt.mark_inactive_leaves = (A gdt).mark_inactive_leaves):
+    Gdt.eval_option (gdt.remove_leaves ((R $ Agdt.map can_prove_empty.val).red.to_finset)) = gdt.eval :=
 begin
     ext env:1,
     
-    -- `A gdt` represents `gdt` by annotating it with refinement types.
+    -- `Agdt` semantically equals `A gdt`, which represents `gdt` by annotating it with refinement types.
+    -- `Agdt` and `A gdt` don't need to be syntactically equal though!
+    -- In fact, `𝒜 gdt` and `A gdt` are semantically equal, but not syntactically.
+
     -- `can_prove_empty` approximates emptiness for a single refinement type.
-    let ant := (A gdt).map can_prove_empty.val,
+    -- `ant_empt` approximates emptiness of the refinement types in `Agdt` for every `env`.
+    -- It also approximates inactive leaves of `gdt` in context of `env` (ant_empt_imp_gdt).
+    let ant_empt := Agdt.map can_prove_empty.val,
+    have ant_empt_imp_gdt := calc
+        ant_empt ⟶ Agdt.mark_inactive_leaves env : can_prove_empty_implies_inactive can_prove_empty Agdt env
+        ...      ⟶ (A gdt).mark_inactive_leaves env : by simp [Ant.implies.refl, ant_def]
+        ...      ⟶ gdt.mark_inactive_leaves env : by simp [Ant.implies.refl, A_mark_inactive_leaves gdt env],
 
-    -- `ant` approximates emptiness of these refinement types for every `env` (s1).
-    have s1: ant ⇒ (A gdt).mark_inactive_leaves env
-        := @can_prove_empty_implies_inactive _ can_prove_empty (A gdt) env,
+    -- Since `gdt` has disjoint leaves, `ant_empt` has disjoint leaves too.
+    have ant_empt_disjoint : ant_empt.disjoint_leaves
+        := by simp [Ant.disjoint_leaves_of_gdt_disjoint_leaves gdt_disjoint,
+                Ant.disjoint_leaves_of_mark_inactive_leaves_eq (function.funext_iff.1 ant_def env)],
 
-    -- Since a refinement type in `A gdt` is empty in `env` iff
-    -- the corresponding leaf- or diverge-node in `gdt` is inactive in `env` (s2),
-    have s2: (A gdt).mark_inactive_leaves env = gdt.mark_inactive_leaves env
-        := A_mark_inactive_leaves gdt env,
-    -- `ant` also approximates inactive leaves of `gdt` in context of `env` (s3).
-    have s3: ant ⇒ gdt.mark_inactive_leaves env
-        := eq.subst s2 s1,
-
-    -- `R_red` is the set we want to remove.
-    let R_red := (R ant).red.to_finset,
-
-    -- The set of leaves `R_red` is redundant in `ant`.
+    -- The set of leaves `R_red` is redundant in `ant_empt` (red_in_ant_empt).
     -- This means that these leaves are inactive
-    -- and possibly active diverge nodes are not removed.
-    have s4: R_red.redundant_in ant 
-        := R_red_redundant ant,
+    -- and not all leaves of possibly active diverge nodes are redundant.
+    let R_red := (R ant_empt).red.to_finset,
+    have red_in_ant_empt: R_red.redundant_in ant_empt := R_red_redundant ant_empt_disjoint,
     
-    -- Since `redundant` is monotonous and `ant` approximates inactive leaves on `gdt`,
-    -- `R_red` can also be removed from `gdt` (s5).
-    have s5: R_red.redundant_in (gdt.mark_inactive_leaves env)
-        := redundant_in.monotonous _ s3 s4,
+    -- Since `redundant_in` is monotonous and `ant_empt` approximates inactive leaves on `gdt`,
+    -- `R_red` is also redundant in `gdt` (red_in_gdt).
+    have red_in_gdt: R_red.redundant_in (gdt.mark_inactive_leaves env)
+        := redundant_in.monotonous _ ant_empt_imp_gdt red_in_ant_empt,
     
     -- Since `R_red` is a redundant set, it can be removed from `gdt` without
     -- changing the semantics. Note that `R_red` is independent of env.
-    have s6: Gdt.eval_option (Gdt.remove_leaves R_red gdt) env = gdt.eval env
-        := redundant_leaves_removable gdt gdt_disjoint env _ s5,
+    have this: Gdt.eval_option (Gdt.remove_leaves R_red gdt) env = gdt.eval env
+        := redundant_leaves_removable gdt gdt_disjoint env _ red_in_gdt,
 
     -- This finishes the proof.
-    exact s6,
+    exact this,
+end
+
+lemma r_correct_1 (ant: Ant bool):
+    (R ant).inacc.to_finset ∪ (R ant).red.to_finset ⊆ ant.inactive_leaves :=
+begin
+    induction ant,
+    case Ant.leaf {
+        cases c: ant_a;
+        simp [R, c, Ant.inactive_leaves],
+    },
+    case Ant.branch {
+        simp [R, Ant.inactive_leaves, *],
+        have := finset.union_subset_union ant_ih_tr1 ant_ih_tr2,
+        simp [finset.union_comm, finset.union_assoc, finset.union_left_comm] at this,
+        exact this,
+    },
+    case Ant.diverge {
+        cases (R_diverge_cases ant_tr ant_a);
+        rw h_R,
+        case R_diverge_case.case1 {
+            simp [h_R_ant, finset.insert_eq] at ant_ih,
+            simp [R, Ant.inactive_leaves, ant_ih],
+        },
+        case R_diverge_case.case2 {
+            simp [Ant.inactive_leaves, ant_ih],
+        },
+    }
+end
+
+lemma disjoint_sets { α: Type } [decidable_eq α] { a₁ a₂ b₁ b₂: finset α } (h: disjoint b₁ b₂) (h₁: a₁ ⊆ b₁) (h₂: a₂ ⊆ b₂):
+    (b₁ ∪ b₂) \ (a₁ ∪ a₂) = (b₁ \ a₁) ∪ (b₂ \ a₂) :=
+begin
+    rw finset.subset_iff at h₁,
+    rw finset.subset_iff at h₂,
+    rw finset.ext_iff,
+    assume a,
+    specialize @h₁ a,
+    specialize @h₂ a,
+    rw finset.disjoint_iff_inter_eq_empty at h,
+    rw finset.ext_iff at h,
+    specialize @h a,
+    
+    finish,
+end
+
+lemma gdt_mark_inactive_leaves_inactive_leaves_of_diverged_or_no_match { gdt: Gdt } { env: Env }:
+    (gdt.mark_inactive_leaves env).inactive_leaves = gdt.leaves ↔ gdt.eval env = Result.diverged ∨ gdt.eval env = Result.no_match :=
+begin
+    induction gdt with leaf generalizing env,
+    case Gdt.leaf {
+        simp [Gdt.eval, Gdt.mark_inactive_leaves, Ant.inactive_leaves, Gdt.leaves, ne.symm (finset.singleton_ne_empty leaf)],
+    },
+    case Gdt.grd {
+        cases gdt_grd,
+        case Grd.xgrd {
+            cases c: xgrd_eval gdt_grd env,
+            { simp [Gdt.leaves, grd_eval_xgrd_none c, Gdt.mark_inactive_leaves, c], },
+            { simp [Gdt.leaves, grd_eval_xgrd_some c, Gdt.mark_inactive_leaves, *], },
+        },
+        case Grd.bang {
+            cases c: is_bottom gdt_grd env,
+            { simp [Gdt.leaves, grd_eval_bang_not_bottom c, Gdt.mark_inactive_leaves, Ant.inactive_leaves, *], },
+            { simp [Gdt.leaves, grd_eval_bang_bottom c, Gdt.mark_inactive_leaves, Ant.inactive_leaves, c], },
+        }
+    },
+    case Gdt.branch {
+        simp [Gdt.mark_inactive_leaves, Ant.inactive_leaves],
+        by_cases c: gdt_tr1.eval env = Result.no_match;
+        simp [c, Gdt.leaves],
+        {
+            rw ←gdt_ih_tr2,
+            rw Gdt.mark_inactive_leaves_no_match c,
+            rw Gdt.mark_all_leaves_inactive.inactive_leaves,
+            sorry,
+        }, {
+            sorry,
+        }
+    },
+end
+
+lemma gdt_mark_inactive_leaves_inactive_leaves_of_leaf_match { gdt: Gdt } { env: Env } { leaf: Leaf } (gdt_disjoint: gdt.disjoint_leaves):
+    gdt.leaves \ (gdt.mark_inactive_leaves env).inactive_leaves = { leaf } ↔ gdt.eval env = Result.leaf leaf :=
+begin
+    induction gdt with l generalizing env,
+    case Gdt.leaf {
+        simp [Gdt.eval, Gdt.mark_inactive_leaves, Ant.inactive_leaves, Gdt.leaves, finset.singleton_inj],
+    },
+    case Gdt.grd {
+        unfold Gdt.disjoint_leaves at gdt_disjoint,
+        cases gdt_grd,
+        case Grd.xgrd {
+            cases c: xgrd_eval gdt_grd env,
+            { simp [Gdt.leaves, grd_eval_xgrd_none c, Gdt.mark_inactive_leaves, c, ne.symm (finset.singleton_ne_empty _)], },
+            { simp [Gdt.leaves, grd_eval_xgrd_some c, Gdt.mark_inactive_leaves, @gdt_ih gdt_disjoint val, *], },
+        },
+        case Grd.bang {
+            cases c: is_bottom gdt_grd env,
+            { simp [Gdt.leaves, grd_eval_bang_not_bottom c, Gdt.mark_inactive_leaves, Ant.inactive_leaves, *], },
+            { simp [Gdt.leaves, grd_eval_bang_bottom c, Gdt.mark_inactive_leaves, Ant.inactive_leaves, c, @gdt_ih gdt_disjoint env, ne.symm (finset.singleton_ne_empty _)], },
+        },
+    },
+    case Gdt.branch {
+        unfold Gdt.disjoint_leaves at gdt_disjoint,
+        replace gdt_ih_tr1 := λ env, @gdt_ih_tr1 gdt_disjoint.1 env,
+        replace gdt_ih_tr2 := λ env, @gdt_ih_tr2 gdt_disjoint.2.1 env,
+
+        simp only [Gdt.leaves, Gdt.mark_inactive_leaves, Ant.inactive_leaves, ne.def],
+
+        have x : (gdt_tr1.mark_inactive_leaves env).inactive_leaves ⊆ gdt_tr1.leaves :=
+        begin
+            rw ←Gdt.mark_inactive_leaves.leaves,
+            exact Ant.inactive_leaves_subset_leaves,
+        end,
+        have y : (
+                if ((gdt_tr1.eval env).is_match)
+                then gdt_tr2.mark_all_leaves_inactive
+                else (gdt_tr2.mark_inactive_leaves env)
+            ).inactive_leaves ⊆ gdt_tr2.leaves := 
+        begin
+            cases (gdt_tr1.eval env).is_match,
+            case bool.ff {
+                rw ←Gdt.mark_inactive_leaves.leaves _ env,
+                simp only [if_false, bool.coe_sort_ff, Ant.inactive_leaves_subset_leaves],
+            },
+            case bool.tt {
+                rw ←Gdt.mark_all_leaves_inactive.leaves,
+                simp only [if_true, bool.coe_sort_tt, Ant.inactive_leaves_subset_leaves],
+            },
+        end,
+
+        rw disjoint_sets gdt_disjoint.2.2 x y,
+        rw Gdt.eval_branch_match_2,
+        rw ←gdt_ih_tr2,
+        rw ←gdt_ih_tr1,
+        
+        cases c: (gdt_tr1.eval env).is_match, {
+            simp at c,
+            simp [c, gdt_mark_inactive_leaves_inactive_leaves_of_diverged_or_no_match.2 (or.inr c), ne.symm (finset.singleton_ne_empty _)],
+        }, {
+            simp at c,
+            simp [c],
+        }
+    },
+end
+
+lemma Gdt.eval.leaf_mem_leaves { gdt: Gdt } { env: Env } { leaf: Leaf } (h: gdt.eval env = Result.leaf leaf): leaf ∈ gdt.leaves :=
+begin
+    induction gdt with leaf generalizing env,
+    case Gdt.leaf {
+        finish [Gdt.leaves, Gdt.eval],
+    },
+    case Gdt.grd {
+        cases gdt_grd,
+        case Grd.xgrd {
+            cases c: xgrd_eval gdt_grd env,
+            { finish [Gdt.leaves, grd_eval_xgrd_none c, Gdt.eval], },
+            { finish [Gdt.leaves, grd_eval_xgrd_some c, Gdt.eval], },
+        },
+        case Grd.bang {
+            cases c: is_bottom gdt_grd env,
+            { finish [Gdt.leaves, grd_eval_bang_not_bottom c], },
+            { finish [Gdt.leaves, grd_eval_bang_bottom c], },
+        }
+    },
+    case Gdt.branch {
+        by_cases c: gdt_tr1.eval env = Result.no_match;
+        finish [Gdt.leaves,  Gdt.eval_branch_match_2],
+    },
+end
+
+lemma f__oo { gdt: Gdt } { env: Env } { leaf: Leaf } { ant: Ant bool }
+    (gdt_disjoint: gdt.disjoint_leaves)
+    (can_prove_empty: Gs)
+    (ant_def: (A gdt).mark_inactive_leaves env = ant)
+    (h: gdt.eval env = Result.leaf leaf):
+    leaf ∈ (R ant).acc \ ((R ant).inacc ++ (R ant).red) :=
+begin
+    rw ←gdt_mark_inactive_leaves_inactive_leaves_of_leaf_match gdt_disjoint at h,
+    rw A_mark_inactive_leaves gdt env at ant_def,
+    rw ant_def at h,
+
+    have : leaf ∉ ant.inactive_leaves :=
+    begin
+        rw finset.ext_iff at h,
+        specialize h leaf,
+        simp at h,
+        exact h.2,
+    end,
+
+    have x : leaf ∉ (R ant).inacc ++ (R ant).red :=
+    begin
+        have := r_correct_1 ant,
+        rw finset.subset_iff at this,
+        specialize @this leaf,
+        finish,
+    end,
+    
+    have : leaf ∈ (R ant).acc :=
+    begin
+        have ant_disjoint: ant.disjoint_leaves := by sorry,
+        have := (R_red_partition ant_disjoint).1,
+        have l : leaf ∈ ant.leaves := by sorry,
+        rw ←this at l,
+        simp at x,
+        push_neg at x,
+        simp [x] at l,
+        exact l,
+    end,
+
 end
