lean/src/internal/utils.lean
@@ -17,6 +17,13 @@ begin
     finish [this],
 end
 
+lemma subset_left_union { α: Type } [decidable_eq α] { u v w: finset α } (h: u ⊆ w): u ⊆ v ∪ w :=
+begin
+    have : ∅ ⊆ v := by simp,
+    have := finset.union_subset_union this h,
+    finish [this],
+end
+
 lemma subset_union_right_subset { α: Type } [decidable_eq α] { u v w: finset α } (h: u ∪ v ⊆ w): u ⊆ w :=
 begin
     rw finset.subset_iff,
